src/LinSimpl.v
@@ -1,0 +1,130 @@
+Set Implicit Arguments.
+Require Import ZArith Psatz.
+Require Import Znumtheory.
+Require Import List Sorting Permutation.
+Require Import MiniCooper.MyTactics.
+Import ListNotations.
+Open Scope list_scope.
+Open Scope Z_scope.
+
+(* Normalization procedure on linear combinations. *)
+
+Module Type LinVar.
+  Parameter t : Type.
+  Parameter eqdec : forall (v1 v2 : t), { v1 = v2 } + { v1 <> v2 }.
+  Parameter leb : t -> t -> bool.
+  Parameter leb_total : forall a b, is_true (leb a b) \/ is_true (leb b a).
+End LinVar.
+
+Module LinSimpl (Var : LinVar).
+
+(* A monom is a variable multiplied by a constant coefficient *)
+Notation monom := (Var.t * Z)%type.
+
+(* A linear combination is a list of monoms, and should be interpreted as their
+   sum. *)
+Definition lin := list monom.
+
+Definition clear_zeros (l : lin) : lin :=
+  filter (fun '(v, k) => negb (Z.eqb k 0)) l.
+
+(* Compaction: merges coefficients of monoms with the same variable.
+   This assumes [l] to be sorted. *)
+Fixpoint compact_with (m : monom) (l : lin) : lin :=
+  let '(v, k) := m in
+  match l with
+  | [] =>
+    [m]
+  | (v', k') :: l' =>
+    if Var.eqdec v v' then
+      compact_with (v, k + k') l'
+    else
+      m :: compact_with (v', k') l'
+  end.
+
+Definition compact (l : lin) : lin :=
+  match l with
+  | [] =>
+    []
+  | m :: l' =>
+    compact_with m l'
+  end.
+
+Module MonomOrder <: Orders.TotalLeBool.
+  Definition t := monom.
+  Definition leb (x y : t) := Var.leb (fst x) (fst y).
+  Lemma leb_total : forall a b, is_true (leb a b) \/ is_true (leb b a).
+  Proof.
+    destruct a, b; unfold leb; simpl.
+    destruct (Var.leb_total t0 t1); eauto.
+  Qed.
+End MonomOrder.
+
+Module MonomSort := Sort MonomOrder.
+
+Definition simpl (l : lin) : lin :=
+  let l := MonomSort.sort l in
+  let l := compact l in
+  clear_zeros l.
+
+(* ------------------------------------------------------------------------- *)
+
+Definition interpret_lin (var : Var.t -> Z) (l : lin) : Z :=
+  fold_right (fun '(v, k) acc =>
+    acc + k * var v
+  ) 0 l.
+
+Local Ltac rew :=
+  rewrite
+     ?Nat.eqb_eq, ?Nat.eqb_neq,
+     ?Bool.negb_false_iff, ?Bool.negb_true_iff,
+     ?Z.eqb_eq, ?Z.eqb_neq
+  in *.
+
+Lemma interpret_clear_zeros:
+  forall var l,
+  interpret_lin var (clear_zeros l) = interpret_lin var l.
+Proof.
+  induction l as [| [? ?]]; intros; simpl in *; eauto.
+  case_if; simpl; rew; subst; lia.
+Qed.
+
+Lemma interpret_compact_with:
+  forall var l k v,
+  interpret_lin var (compact_with (v,k) l) =
+  k * var v + interpret_lin var l.
+Proof.
+  induction l as [| [? ?]]; intros; simpl in *; eauto.
+  case_if; simpl; rewrite IHl; rew; subst; nia.
+Qed.
+
+Lemma interpret_compact:
+  forall var l,
+  interpret_lin var (compact l) = interpret_lin var l.
+Proof.
+  intros. unfold compact. destruct l as [|[? ?]]; eauto.
+  rewrite interpret_compact_with. simpl. nia.
+Qed.
+
+Lemma interpret_lin_permutation:
+  forall var l1 l2,
+  Permutation l1 l2 ->
+  interpret_lin var l1 = interpret_lin var l2.
+Proof.
+  introv HP. induction HP;
+  repeat match goal with x: (_ * _)%type |- _ => destruct x end;
+  simpl; auto.
+Qed.
+
+Lemma interpret_simpl:
+  forall var l,
+  interpret_lin var (simpl l) =
+  interpret_lin var l.
+Proof.
+  intros. unfold simpl.
+  rewrite interpret_clear_zeros, interpret_compact.
+  rewrite interpret_lin_permutation with (l1:=l) (l2:=(MonomSort.sort l));
+  auto using MonomSort.Permuted_sort.
+Qed.
+
+End LinSimpl.
